Index_spec done. Loops for resize done. resize begun, but missing proof of population size.

iterators/hashtable.v
@@ -1,6 +1,6 @@
 From iris.proofmode Require Import tactics.
-From iris.prelude Require Import list gmap.
-From iris.heap_lang Require Import notation proofmode.
+From iris.heap_lang Require Import lang notation proofmode.
+From iris.prelude Require Import list.
 From iris.program_logic Require Import hoare.
 
 Close Scope Z_scope.
@@ -21,11 +21,11 @@ Section HashTable.
 
   Hypothesis array_load_spec:
     forall arr xs v (n : nat),
-      xs !! n = Some v -> {{array arr xs}} array_load (arr, #n) {{u, ⌜u = v⌝ ∗ array arr xs}}%I.
+      xs !! n = Some v -> {{{array arr xs}}} array_load (arr, #n) {{{ RET v;array arr xs}}}.
 
   Hypothesis array_store_spec:
     forall arr xs (v : val) (n : nat),
-      n < length xs -> {{array arr xs}} array_store (arr, #n, v) {{_, array arr (<[n := v]> xs)}}%I.
+      n < length xs -> {{{array arr xs}}} array_store (arr, #n, v) {{{ RET #() ; array arr (<[n := v]> xs)}}}.
 
   Notation "e1 .[ e2 ]" := (array_load (e1, e2)%E) (at level 20): expr_scope.
   Notation "e1 .[ e2 ] := e3" := (array_store (e1, e2, e3)%E) (at level 20): expr_scope.
@@ -72,24 +72,27 @@ Section HashTable.
     Definition index : val :=
       λ: "t" "k", modulo (hash K "k", !(Snd "t")).
 
+
+    Definition mv_buck : val :=
+      rec: "mv_buck" "p" :=
+        let: "t" := Fst "p" in
+        let: "b" := Snd "p" in
+        match: "b" with
+          NONE => #()
+        | SOME "a"
+          => let: "k" := Fst (Fst "a") in
+             let: "x" := Snd (Fst "a") in
+             let: "b'" := Snd "a" in
+             "mv_buck" ("t", "b'");;
+             let: "idx" := index "t" "k" in
+             (!(Fst (Fst "t"))).["idx"] := SOME ("k", "x", (!(Fst (Fst "t"))).["idx"])
+        end.
+    
     Definition resize_loop : val :=
-      rec: "loop" "cap" "old" "t" "i" :=
+      rec: "loop" "i" "cap" "old" "t" :=
                    if: "i" < "cap" then
-                     let: "mv_buck" :=
-                        rec: "mv_buck" "b" :=
-                          match: "b" with
-                            NONE => #()
-                          | SOME "a"
-                            => let: "k" := Fst (Fst "a") in
-                               let: "x" := Snd (Fst "a") in
-                               let: "b'" := Snd "a" in
-                               "mv_buck" "b'";;
-                               let: "idx" := index "t" "k" in
-                               (!(Fst (Fst "t"))).["idx"] := SOME ("k", "x", (!(Fst (Fst "t"))).["idx"])
-                          end
-                     in
-                     "mv_buck" ("old".["i"]);;
-                     "loop" ("i" + #1)
+                     mv_buck ("t", ("old".["i"]));;
+                     "loop" ("i" + #1) "cap" "old" "t"
                    else #().
 
     Definition resize : val :=
@@ -97,7 +100,7 @@ Section HashTable.
               let: "cap" :=  !(Snd "t") in
               Fst (Fst "t") <- make_array ("cap" + "cap", NONE);;
               Snd "t" <- "cap" + "cap";;
-              resize_loop "cap" "old" "t" #0.
+              resize_loop #0 "cap" "old" "t".
     
     Definition resize2 : val :=
       λ: "t", let: "old" := !(Fst (Fst "t")) in
@@ -215,13 +218,54 @@ Section HashTable.
       rewrite list_lookup_insert_ne ; [|done].
       by unfold lookupData.
     Qed.
-      
+
+    Lemma list_fmap_insert `(f: A -> B) (l : list A) i x :
+      f <$> (<[i := x]> l) = <[i := f x]> (f <$> l).
+    Proof.
+      revert i.
+      induction l as [| y l' IH] ; [done|].
+      intros [|i] ; [done|].
+      csimpl.
+      by rewrite IH.
+    Qed.
+
+    Lemma sum_list_with_lookup `(f: A -> nat) l i x :
+      (l !! i) = Some x ->
+      f x ≤ sum_list_with f l.
+    Proof.
+      revert i.
+      induction l as [|x' l IH] ; [done|].
+      intros [|i].
+      - simpl.
+        intro.
+        simplify_eq.
+        lia.
+      - simpl.
+        intro Hlookup.
+        pose proof (IH _ Hlookup).
+        lia.
+    Qed.
+    
     Definition content M (data : list BucketData) :=
       forall k,
         M k
         = map snd (filter (fun p => as_key K (p.1) = Some k)
                           (lookupData data k)).
 
+    Lemma content_empty n :
+      content (const []) (replicate n []).
+    Proof.
+      intro k.
+      unfold lookupData.
+      destruct (decide (0 = n)) as [<-|].
+      done.
+      rewrite lookup_replicate_2.
+      done.
+      rewrite replicate_length.
+      apply mod_bound_pos ; lia.
+    Qed.
+      
+      
     Lemma content_insert M data k k' x:
       0 < length data ->
       as_key K k' = Some k ->
@@ -248,18 +292,62 @@ Section HashTable.
         + by rewrite lookup_insert_data_other.
     Qed.
     
+    Definition have_keys (data : list BucketData) :=
+      Forall (fun b => Forall (fun '(k, _) => is_Some (as_key K k)) b) data.
+
+    Lemma have_keys_empty n :
+      have_keys (replicate n []).
+    Proof.
+      apply Forall_forall.
+      intros b HbIn.
+      pose proof (elem_of_replicate n [] b) as Hb.
+      setoid_rewrite Hb in HbIn.
+      inversion HbIn as [HbNil _].
+      by rewrite HbNil.
+    Qed.      
       
-    
-    
+    Lemma have_keys_insert data k k' x:
+      as_key K k' = Some k ->
+      have_keys data ->
+      have_keys (insertData data k (k', x)).
+    Proof.
+      intros HKey Hdata.
+    (*  unfold insertData.
+      unfold have_keys.
+      unfold lookupData.
+      eauto using Forall_insert, Forall_lookup, Forall_cons. *)
+      apply Forall_insert ; [assumption|].
+      apply Forall_cons.
+      split.
+      by exists k.
+      unfold lookupData.
+      destruct (decide ((Hash K k mod length data) < length data)) as [Hlt|Hge].
+      destruct (lookup_lt_is_Some_2 _ _ Hlt) as [b Hb].
+      rewrite Hb. simpl.
+      apply (Forall_lookup_1 _ _ _ _ Hdata Hb).
+      rewrite (lookup_ge_None_2 _ _). by simpl.
+      assert (forall n m, n <= m <-> ~ m < n) as tmp. intros. lia.
+      by apply tmp.
+    Qed.
+      
+      
     Definition no_garbage (data : list BucketData) :=
       forall i k,
         i < length data -> 
         i ≠ Hash K k mod length data ->
-        [] = map snd (filter (fun p => as_key K (p.1) = Some k)
+        [] = snd <$> (filter (fun p => as_key K (p.1) = Some k)
                              (from_option
                                 id []
                                 (data !! i))).
 
+    Lemma no_garbage_empty n :
+      no_garbage (replicate n []).
+    Proof.
+      intros i k Hi _.
+      rewrite lookup_replicate_2 ; [done|].
+      by rewrite replicate_length in Hi.
+    Qed.
+      
     Lemma no_garbage_insert data k k' x :
       as_key K k' = Some k ->
       no_garbage data ->
@@ -283,16 +371,29 @@ Section HashTable.
       - rewrite list_lookup_insert_ne ; [|done].
         apply HNG ; done.
     Qed.
+
+    (*
+    Lemma size_equivalence M data data' :
+      content M data ->
+      no_garbage data ->
+      have_keys data ->
+      content M data' ->
+      no_garbage data' ->
+      have_keys data' ->
+      sum_list_with length data = sum_list_with length data'.
+    Proof.
+      *)
       
     Definition TableInState M (lData : loc) (data: list BucketData) (t : val) : iProp Σ:=
       ( ⌜length data > 0⌝ ∗
         ⌜content M data⌝ ∗
         ⌜no_garbage data⌝ ∗
+        ⌜have_keys data⌝ ∗
         ∃ (lSize lCap : loc) arr,
           ⌜t = (#lData, #lSize, #lCap)%V⌝ ∗
           array arr (fmap bucket data) ∗
           lData ↦ arr ∗
-          lSize ↦ #(fold_right (fun l a => a + length l) 0 data)%nat ∗
+          lSize ↦ #(sum_list_with length data)%nat ∗
           lCap ↦ #(length data))%I.
 
     Definition Table M (t : val) : iProp Σ :=
@@ -307,6 +408,35 @@ Section HashTable.
       reflexivity.
     Qed.
 
+    (*
+    Notation "'for:' i := e1 'to' e2 'do' e3" :=
+      (Lam "__$for_begin$__"
+           (Lam "__$for_end$__" 
+                (Rec "__$for_loop$__" (BNamed i%string)
+                     (If (BinOp LtOp (Var i) "__$for_end$__" )
+                         (Let BAnon e3%E ("__$for_loop$__" (BinOp PlusOp (Var i) (Lit (LitInt 1)))))
+                         (Lit LitUnit))
+                     "__$for_begin$__$")
+                e2%E)
+           e1%E)
+        (at level 200, i at level 1, e1, e2, e3 at level 200) : expr_scope.
+
+    Lemma wp_for E m n e en j P:
+      (m ≤ n)%Z ->
+      Closed [j] e ->
+      Closed [] en ->
+      WP en @ E {{v, ⌜v = #n⌝}} -∗ P m -∗
+         (∀ (i : Z), ⌜m ≤ i < n⌝%Z -∗ P i -∗ ▷ WP (subst' j #i e) @ E {{_, P (i + 1)%Z}}) -∗
+         WP for: j := #m to en do e @ E {{_, P n}}.
+    Proof.
+      intros Hle HClosede HCloseden.
+      iIntros "HWPen HPm Hinv".
+      iApply wp_lam.
+      reflexivity.
+      exists #m.
+      done.
+      *)
+      
     Lemma create_impl_spec n : n > 0 -> WP create_impl #n {{t, Table (const []) t}}%I.
     Proof.
       intro Hn.
@@ -320,27 +450,10 @@ Section HashTable.
       wp_alloc lCap as "HlCap".
       iExists lArr, (replicate n []).
 
-      iSplit.
-      iPureIntro. by rewrite replicate_length.
-      iSplit.
-      iPureIntro.
-      intro k.
-      simpl.
-      unfold lookupData.
-      rewrite replicate_length.
-      assert (Hash K k `mod` n < n).
-      { intros. apply Nat.mod_upper_bound. unfold gt in Hn. Nat.order. }
-      assert ((replicate n [] !! (Hash K k `mod` n)) = Some ([] : BucketData)) as HSome.
-      { intros. by rewrite lookup_replicate. }
-      by rewrite HSome.
-      iSplit.
-      iPureIntro.
-      intros i k.
-      rewrite replicate_length.
-      intros Hi _.
-      assert (replicate n [] !! i = Some ([] : BucketData)) as HSome.
-      { by rewrite lookup_replicate. }
-      by rewrite HSome.
+      iSplit. iPureIntro. by rewrite replicate_length.
+      iSplit. iPureIntro. apply content_empty.
+      iSplit. iPureIntro. apply no_garbage_empty.
+      iSplit. iPureIntro. apply have_keys_empty.
       iExists lSize, lCap, arr.
       iSplit. done.
       iSplitL "Harr".
@@ -348,13 +461,13 @@ Section HashTable.
       iFrame.
       iSplitL "HlSize".
       clear Hn.
-      assert (0 = foldr (λ (l : list (val * val)) (a : nat), a + length l) 0 (replicate n [])) as Hsize.
+      assert (0 = sum_list_with length (replicate n ([] : BucketData))) as Hsize.
       { induction n as [|n IH]. done. simpl. by rewrite -IH. }
       by rewrite -Hsize.
       by rewrite replicate_length.
     Qed.
 
-    Lemma index_spec (lArr lSize lCap : loc) (k : val) M k' (data : list val) :
+    Lemma index_spec (lArr lSize lCap : loc) (k : val) k' (data : list val) :
       as_key K k = Some k' -> {{{lCap ↦ #(length data)}}} index (#lArr, #lSize, #lCap) k {{{RET #(Hash K k' mod length data)%nat ; lCap ↦ #(length data)}}}.
     Proof.
       intro HKey.
@@ -395,34 +508,191 @@ Section HashTable.
       by iFrame.
     Qed.*)
 
-(* Uncommented for now as loops are hard to handle.
-
-    Lemma resize_loop_spec M M' data data' old new lArr lSize lCap i : 
+        
+    Lemma mv_buck_spec M data arr (lArr lSize lCap : loc) b :
       content M data ->
-      content M' data' ->
-      (forall k, M' !! k = if decide (Hash K k mod length data' < i)
-                           then M !! k
-                           else None) ->
-      exists data'',
-        content M data'' /\
-        {{{lArr ↦ new ∗ lCap ↦ #(length data') ∗ array new (map bucket data')∗ array old (map bucket data) }}}
-          resize_loop #(length data) old (#lArr, #lSize, #lCap) #i
-          {{{ RET #(); lArr ↦ new ∗ lCap ↦ #(length data'') ∗ array new (map bucket data'')∗ array old (map bucket data)}}}.
+      no_garbage data ->
+      have_keys data ->
+      0 < length data ->
+      Forall (fun '(k, x) => is_Some (as_key K k)) b ->  
+      {{{ array arr (bucket <$> data) ∗ lArr ↦ arr ∗ lCap ↦ #(length data) }}}
+        mv_buck ((#lArr, #lSize, #lCap), (bucket b))
+        {{{ M' data', RET #() ; array arr (bucket <$> data') ∗
+                                lArr ↦ arr ∗
+                                lCap ↦ #(length data') ∗
+                                ⌜∀ k, M' k =
+                                      (snd <$> (filter (fun p => as_key K (p.1) = Some k)
+                                                       b)) ++ M k⌝ ∗
+                                ⌜content M' data'⌝ ∗
+                                ⌜no_garbage data'⌝ ∗
+                                ⌜have_keys data'⌝ ∗
+                                ⌜length data = length data' ⌝}}}.
     Proof.
-      intros Hdata.
-      iLöb as "IH" forall (i).
-      Hdata' HM'.
-      eexists.
-      split; last first.
-      iIntros (Φ) "[HlArr [HlCap [Hnew Hold]]] HΦ".
-      iRevert (M' data') "Hnew HΦ".
-      
-      
+      intros HContent HNG HKeys Hlen.
+      induction b as [|(k', x) b IH].
+      - iIntros (_ Φ) "[Harr [HlArr HlCap]] HΦ".
+        wp_rec.
+        wp_proj.
+        wp_lam.
+        wp_proj.
+        wp_lam.
+        wp_match.
+        iApply "HΦ".
+        iFrame.
+        eauto.
+      - iIntros (HKey Φ) "HPre HΦ".
+        inversion HKey as [|tmp tmp2 HKeyk HKeyb].
+        destruct HKeyk as [k HKeyk].
+        wp_rec.
+        wp_proj.
+        wp_lam.
+        wp_proj.
+        wp_lam.
+        wp_match.
+        do 2 wp_proj.
+        wp_lam.
+        do 2 wp_proj.
+        wp_lam.
+        wp_proj.
+        wp_lam.
+        wp_apply (IH _ with "HPre").
+        iIntros (M' data') "[Harr [HlArr [HlCap [% [% [% [% %]]]]]]]".
+        rename H6 into HLenEq.
+        wp_lam.
+        wp_apply (index_spec _ _ _ _ k (bucket <$> data) _ with "[HlCap]").
+        rewrite fmap_length. rewrite HLenEq. iFrame.
+        iIntros "HlCap".
+        wp_lam.
+        do 2 wp_proj.
+        wp_load.
+        do 2 wp_proj.
+        wp_load.
+        assert (Hash K k `mod` length (bucket <$> data) < length data') as HLenFmap.
+        { rewrite -HLenEq. rewrite fmap_length. apply mod_bound_pos. lia. done. }
+        assert (exists l, data' !! (Hash K k `mod` length (bucket <$> data)) = Some l) as HSome.
+        by apply lookup_lt_is_Some_2.
+        destruct HSome as [l HSome].
+        pose proof (list_lookup_fmap bucket data' (Hash K k `mod` length (bucket <$> data))) as HBucket.
+        rewrite HSome in HBucket.
+        simpl in HBucket.
+        wp_apply (array_load_spec _  _ _ _ HBucket with "Harr").
+        iIntros "Harr".
+        rewrite -(fmap_length bucket) in HLenFmap.
+        wp_apply (array_store_spec _ _ (SOMEV (k', x, bucket l)) _ HLenFmap with "Harr").
+        iIntros "Harr".
+        iApply ("HΦ" $! (<[k := x]> M') (insertData data' k (k',x))).
+        iSplitL "Harr".
+        rewrite list_fmap_insert.
+        unfold lookupData.
+        rewrite fmap_length HLenEq in HSome.
+        rewrite HSome.
+        simpl.
+        rewrite fmap_length HLenEq.
+        iApply "Harr".
+        iFrame.
+        iSplit.
+        unfold insertData.
+        by rewrite insert_length fmap_length HLenEq.
+        iSplit. iPureIntro.
+        intro k''.
+        simpl.
+        unfold filter. unfold list_filter. unfold base.insert. unfold insertM. simpl. rewrite HKeyk.
+        destruct (decide (k = k'')) as [<-|].
+        rewrite decide_True ; [|reflexivity]. 
+        simpl. by f_equal.
+        rewrite decide_False ; [done | by injection].
+        iSplit. iPureIntro.
+        apply content_insert ; [by rewrite -HLenEq|assumption..].
+        iSplit. iPureIntro.
+        apply no_garbage_insert ; assumption.
+        iSplit. iPureIntro.
+        apply have_keys_insert ; assumption.
+        iPureIntro.
+        unfold insertData. rewrite HLenEq. symmetry. apply insert_length.
+        Unshelve. assumption.
+        assumption.
+    Qed.        
+
+    
+    Lemma resize_loop_spec M data data' old new (lArr lSize lCap : loc) i : 
+      content M data ->
+      no_garbage data ->
+      have_keys data ->
+      0 < length data -> 
+      content (fun k => if decide (Hash K k mod length data < i)
+                           then M k
+                        else [])  data' ->
+      no_garbage data' ->
+      have_keys data' ->
+      0 < length data' -> 
+      {{{lArr ↦ new ∗ lCap ↦ #(length data') ∗ array new (bucket <$> data')∗ array old (bucket <$> data) }}}
+        resize_loop #i #(length data) old (#lArr, #lSize, #lCap)
+        {{{ data'', RET #(); lArr ↦ new ∗
+                            lCap ↦ #(length data'') ∗
+                            array new (map bucket data'') ∗
+                            array old (map bucket data) ∗
+                            ⌜content M data''⌝ ∗
+                            ⌜no_garbage data''⌝ ∗
+                            ⌜have_keys data''⌝ ∗
+                            ⌜length data'' = length data'⌝ }}}.
+    Proof.
+      intros HContentData HNGdata HKeysData HLenData HContentData' HNGdata' HKeysData' HLenData'.
+      intro Φ.
+      iLöb as "IH" forall (i data' HContentData' HNGdata' HKeysData' HLenData').
+      iIntros "[HlArr [HlCap [Hnew Hold]]] HΦ".
+      wp_rec.
+      do 3 wp_lam.
+      wp_op.
+      - intro Hlt.
+        assert (exists b, data !! i = Some b) as HSome.
+        { apply lookup_lt_is_Some_2. lia. }
+        destruct HSome as [b HSome].
+        wp_if.
+        assert ((bucket <$> data) !! i = Some (bucket b)) as HSomeBucket.
+        { by rewrite list_lookup_fmap HSome. }
+        wp_apply (array_load_spec _ _ _ _ HSomeBucket with "Hold").
+        iIntros "Hold".
+        pose proof (Forall_lookup_1 _ _ _ _ HKeysData HSome) as HKeysb.
+        wp_apply (mv_buck_spec _ _ new lArr lSize lCap _ HContentData' HNGdata' HKeysData' HLenData' HKeysb with "[Hnew HlArr HlCap]").
+        iFrame.
+        iIntros (M'' data'') "[Hnew [HlArr [HlCap [% [% [% [% %]]]]]]]".        
+        wp_lam.
+        wp_op.
+        rewrite (_ : (i+1)%Z = (S i)) ; [|lia].
+        assert (content (λ k : Key K, if decide (Hash K k `mod` length data < S i) then M k else []) data'') as HContentData''.
+        { intro k.
+          destruct (decide (Hash K k mod length data < S i)).
+          + rewrite -H1 H0.
+            destruct (decide (Hash K k mod length data < i)).
+            * rewrite (_ :b = from_option id [] (data !! i)) ; [|by rewrite HSome].
+              rewrite -HNGdata ; [done|lia..].
+            * rewrite (_: i = Hash K k `mod` length data) in HSome ;[|lia].
+              rewrite HContentData. unfold lookupData. 
+              rewrite HSome. symmetry. apply app_nil_r.
+          + rewrite -H1 H0. rewrite decide_False ; [|lia].
+            rewrite (_ :b = from_option id [] (data !! i)) ; [|by rewrite HSome].
+            rewrite -HNGdata ; [done|lia..].
+        }
+        iApply ("IH" $! (S i) data'' with "[%] [%] [%] [%] [HlArr HlCap Hnew Hold]");
+          [assumption..| by rewrite (_: length data'' = length data')| iFrame | ].
+        iNext. rewrite (_: length data'' = length data') ; done.
+      - intro Hge.
+        wp_if.
+        iApply "HΦ".
+        iFrame.
+        iSplit. iPureIntro. 
+        intro k. rewrite -HContentData'. rewrite decide_True ; [reflexivity|].
+        assert (Hash K k `mod` length data < length data). apply mod_bound_pos ; lia. lia.
+        auto.
+    Qed.
+        
+    
+        
     Lemma resize_spec t M :
       {{{Table M t}}} resize t {{{ RET #(); Table M t }}}.
     Proof.
       iIntros (Φ) "HTable HΦ".
-      iDestruct "HTable" as (lData data) "[% [% [% HTable]]]".
+      iDestruct "HTable" as (lData data) "[% [% [% [% HTable]]]]".
       iDestruct "HTable" as (lSize lCap arr) "[% [Harr [HlData [HlSize HlCap]]]]".
       iSimplifyEq.
       wp_lam.
@@ -434,31 +704,74 @@ Section HashTable.
       wp_lam.
       do 2 wp_proj.
       wp_op.
+      rewrite -Nat2Z.inj_add.
       wp_bind (make_array _).
       iApply (wp_wand).
-      rewrite -Nat2Z.inj_add.
       iApply (make_array_spec (length data + length data) NONEV).
       iIntros (newArr) "HnewArr".
       wp_store.
       wp_proj.
       wp_op.
       wp_store.
-      iApply (wp_wand with "[Harr HnewArr]").
+      assert (content (λ k : Key K, if decide (Hash K k `mod` length data < 0) then M k else [])
+                      (replicate (length data + length data) [])) as HContent'.
+      { intro k. setoid_rewrite decide_False ; [|lia].
+        unfold lookupData.
+        rewrite lookup_replicate_2.
+        done.
+        rewrite replicate_length.
+        apply mod_bound_pos ; lia.
+      }
+      wp_apply (resize_loop_spec M data _ _ newArr _ _ _ 0 _ _ _ _ HContent' with "[-HlSize HΦ]").
+      apply no_garbage_empty.
+      apply have_keys_empty.
+      rewrite replicate_length ; lia.
+      rewrite replicate_length -Nat2Z.inj_add.
+      rewrite fmap_replicate.
+      iFrame.
+      iIntros (data'') "[HlData [HlCap [HnewArr [Harr [% [% [% %]]]]]]]".
+      rename H7 into HLen.
+      iApply "HΦ".
+      iExists lData, data''.
+      iSplit. iPureIntro.
+      rewrite HLen replicate_length. lia.
+      iSplit. done.
+      iSplit. done.
+      iSplit. done.
+      iExists lSize, lCap, newArr.
+      iSplit. done.
+      iFrame.
+
+      assert (forall M data data',
+                 content M data ->
+                 no_garbage data ->
+                 have_keys data ->
+                 content M data' ->
+                 no_garbage data' ->
+                 have_keys data' ->
+                 sum_list_with length data = sum_list_with length data').
       
-      rewrite -Nat2Z.inj_0.
-      generalize 0 as i.
-      iIntros (i).
-      iLöb as "IH" forall (i).
       *)
 
-    Lemma list_fmap_insert `(f: A -> B) (l : list A) i x :
-      f <$> (<[i := x]> l) = <[i := f x]> (f <$> l).
-    Proof.
+
+      
+    Lemma sum_list_with_insert `(f : A -> nat) l i x y :
+      (l !! i) = Some y ->
+      sum_list_with f (<[i := x ]> l) =sum_list_with f l + f x - f y .
+    Proof.      
       revert i.
-      induction l as [| y l' IH] ; [done|].
-      intros [|i] ; [done|].
-      csimpl.
-      by rewrite IH.
+      induction l as [|x' l IH].
+      done.
+      intros [|i].
+      simpl.
+      intro.
+      simplify_eq.
+      lia.
+      simpl.
+      intro Hlookup.
+      rewrite IH ; [|done].
+      pose proof (sum_list_with_lookup f _ _ _ Hlookup ).
+      lia.
     Qed.
       
     Lemma insert_impl_spec (t k x : val) M k' :
@@ -466,13 +779,12 @@ Section HashTable.
     Proof.
       intro HKey.
       iIntros (Φ) "HTable HΦ".
-      iDestruct "HTable" as (lArr data) "[% [% [% HTable]]]".
+      iDestruct "HTable" as (lArr data) "[% [% [% [% HTable]]]]".
       iDestruct "HTable" as (lSize lCap arr) "[% [Harr [HlArr [HlSize HlCap]]]]".
       iSimplifyEq.
       do 3 wp_lam.
       wp_bind (index _ _).
-      Check index_spec.
-      wp_apply (index_spec lArr lSize lCap k M k' (fmap bucket data) HKey with "[HlCap]").
+      wp_apply (index_spec lArr lSize lCap k k' (fmap bucket data) HKey with "[HlCap]").
       by rewrite map_length.
       iIntros "HlCap".
       wp_lam.
@@ -485,25 +797,15 @@ Section HashTable.
       assert (exists l, data !! (Hash K k' `mod` length data) = Some l) as HSome.
       by apply lookup_lt_is_Some_2.
       destruct HSome as [l HSome].
-      Check list_lookup_fmap.
       pose proof (list_lookup_fmap bucket data (Hash K k' `mod` length data)) as HBucket.
       rewrite HSome in HBucket.
       simpl in HBucket.
-      iPoseProof  (array_load_spec _ _ _ _ HBucket) as "arrLoadSpec".
-      iDestruct ("arrLoadSpec" with "Harr") as "H".
-      wp_bind (array_load _).
       rewrite fmap_length.
-      iApply (wp_wand with "H") .
-      iIntros (v) "[% Harr]".
-      iSimplifyEq.
-      assert (Hash K k' `mod` length (bucket <$> data) < length (bucket <$> data)) as HLenFmap.
-      by rewrite fmap_length.
-      iPoseProof  (array_store_spec _ _ (SOMEV (k, x, bucket l)) _ HLenFmap) as "arrStoreSpec".
-      iDestruct ("arrStoreSpec" with "Harr") as "H".
-      wp_bind (array_store _).
-      rewrite fmap_length.
-      iApply (wp_wand with "H").
-      iIntros (v) "Harr".
+      wp_apply (array_load_spec _ _ _ _ HBucket with "Harr").
+      iIntros "Harr".
+      rewrite -{2}(fmap_length bucket)  in HLen.
+      wp_apply (array_store_spec _ _ (SOMEV (k, x, bucket l)) _ HLen with "Harr").
+      iIntros "Harr".
       wp_lam.
       do 2 wp_proj.
       wp_load.
@@ -516,15 +818,14 @@ Section HashTable.
       wp_lam.
       iApply "HΦ".
       iExists lArr,  (insertData data k' (k, x)). 
-      iSplit.
-      iPureIntro.
+      iSplit. iPureIntro.
       by rewrite insert_length.
-      iSplit.
-      iPureIntro.
+      iSplit. iPureIntro.
       by apply content_insert.
-      iSplit.
-      iPureIntro.
+      iSplit. iPureIntro.
       by apply no_garbage_insert.
+      iSplit. iPureIntro.
+      apply have_keys_insert ; [assumption|assumption].
       iExists lSize, lCap, arr. 
       iSplit ; [done|].
       iSplitL "Harr".
@@ -537,8 +838,21 @@ Section HashTable.
       iFrame.
       iSplitL "HlSize".
       unfold insertData.
-      
-      
+      unfold lookupData.
+      rewrite HSome.
+      simpl.
+      rewrite (sum_list_with_insert _ _ _ _ _ HSome).
+      simpl.
+      assert (1 + sum_list_with length data =
+              sum_list_with length data + S (length l) - length l) as HLenEq; [lia|].
+      rewrite -(Z2Nat.id 1) ; [|done].
+      rewrite Z2Nat.inj_pos. rewrite Pos2Nat.inj_1. rewrite -inj_plus.
+      rewrite -HLenEq.
+      iFrame.
+      unfold insertData.
+      rewrite insert_length.
+      iFrame.
+    Qed.      
       
   End Implementation.
   
